README.md
@@ -9,6 +9,8 @@ We formalize content from:
 
 # Current state of the project
 
+Something went wrong when I tried updateing the versions of Lean and mathlib on a different branch, hence, dependencies are a bit brocken. I found that a safe way to get the project to run on the correct version is to append `@ "v4.5.0-rc1"` at line 9 of the lakefile, then running `lake update`.
+
 Still a work in progress, though in its final phase.
 I'm currently:
 - Cleaning the content.
@@ -22,10 +24,13 @@ Known related work:
 - https://leanprover-community.github.io/mathlib4_docs/Mathlib/SetTheory/Game/Basic.html
 - https://www.isa-afp.org/entries/GaleStewart_Games.html
 
+
 Please let me know if you're aware of more related work
 
 
 # Roadmap for reading
+
+- I wrote a brief article, to be found in `root > CTarticle` to guide you through the project.
 
 - Start by reading `gameLib > Basic` and `gameLib > Termination`. To see the objects we define there in action, we suggest reading `games > PickUpBricks` on the side, or right after.
 
